Dataflow/WellFormed/Example.v
@@ -11,18 +11,18 @@ Require Import Rustre.Dataflow.IsMemory.
 Require Import Rustre.Dataflow.WellFormed.
 Require Import Rustre.Dataflow.WellFormed.Decide.
 
-Example eqn1_well_sch: Is_well_sch (PS.add 1 (memories eqns1)) eqns1.
+Example eqn1_well_sch: Is_well_sch (memories eqns1) 1 eqns1.
 Proof.
-  assert (well_sch (PS.add 1 (memories eqns1)) eqns1 = true) as HW by apply eq_refl.
-  pose proof (well_sch_spec (PS.add 1 (memories eqns1)) eqns1) as HS.
+  assert (well_sch (memories eqns1) 1 eqns1 = true) as HW by apply eq_refl.
+  pose proof (well_sch_spec (memories eqns1) 1 eqns1) as HS.
   rewrite HW in HS.
   assumption.
 Qed.
 
-Example eqn2_well_sch: Is_well_sch (PS.add 1 (memories eqns2)) eqns2.
+Example eqn2_well_sch: Is_well_sch (memories eqns2) 1 eqns2.
 Proof.
-  assert (well_sch (PS.add 1 (memories eqns2)) eqns2 = true) as HW by apply eq_refl.
-  pose proof (well_sch_spec (PS.add 1 (memories eqns2)) eqns2) as HS.
+  assert (well_sch (memories eqns2) 1 eqns2 = true) as HW by apply eq_refl.
+  pose proof (well_sch_spec (memories eqns2) 1 eqns2) as HS.
   rewrite HW in HS.
   assumption.
 Qed.
